src/proof/delete.v
@@ -17,66 +17,60 @@ Context `{!mapG Σ KKey.t PureKObject.t}.
 Context `{!mapG Σ KKey.t (gset KKey.t)}.
 Context `{!auth_setG Σ KKey.t}.
 
-(* TODO: Revisit this spec and see if owned_grandchild_keys is necessary *)
 Lemma wp_objDelete_pod_ptsto_mut key
-  γ_state γ_children γ_fresh_keys owned_pod parent_key owned_child_keys owned_grandchild_keys:
+  γ_state γ_children γ_fresh_keys pure_pod parent_key owned_child_keys owned_grandchild_keys:
   {{{ is_pkg_init apimodel ∗
-      "#inv" ∷ is_kubernetes_state γ_state γ_children γ_fresh_keys ∗
-      "own_pod" ∷ key [[ γ_state ]]↦ (PureKObject.Pod owned_pod) ∗
-      "own_child_keys" ∷ parent_key [[ γ_children ]]↦ owned_child_keys ∗
-      "own_grandchild_keys" ∷ key [[ γ_children ]]↦ owned_grandchild_keys ∗
-      "%pod_is_child" ∷ ⌜ key ∈ owned_child_keys ⌝ ∗
-      "%kind" ∷ ⌜ KKey.Kind' key = "Pod"%go ⌝
+      "#Hinv" ∷ is_kubernetes_state γ_state γ_children γ_fresh_keys ∗
+      "%Hpod_is_child" ∷ ⌜ key ∈ owned_child_keys ⌝ ∗
+      "%Hkind_is_pod" ∷ ⌜ KKey.Kind' key = "Pod"%go ⌝ ∗
+      "Hown_pod" ∷ key [[ γ_state ]]↦ (PureKObject.Pod pure_pod) ∗
+      "Hown_child_keys" ∷ parent_key [[ γ_children ]]↦ owned_child_keys ∗
+      "Hown_grandchild_keys" ∷ key [[ γ_children ]]↦ owned_grandchild_keys
   }}}
     @! apimodel.objDelete #key
-  {{{ (err: error.t) pod, RET #err;
-      "err_is_nil" ∷ ⌜ err = interface.nil ⌝ ∗
+  {{{ updated_pure_pod, RET #interface.nil;
       "pod_updated_or_deleted" ∷ ("pod_updated" ∷ (
-        "own_pod" ∷ key [[ γ_state ]]↦ (PureKObject.Pod pod) ∗
-        "own_child_keys" ∷ parent_key [[ γ_children ]]↦ owned_child_keys ∗
-        "own_grandchild_keys" ∷ key [[ γ_children ]]↦ owned_grandchild_keys ∗
-        "%deletiontimestamp_notnull" ∷ ⌜ pod.(v1.Pod.ObjectMeta').(v1.ObjectMeta.DeletionTimestamp') ≠ null ⌝
+        "%deletiontimestamp_notnull" ∷ ⌜ updated_pure_pod.(PurePod.ObjectMeta').(PureObjectMeta.DeletionTimestamp') ≠ None ⌝ ∗
+        "Hown_pod" ∷ key [[ γ_state ]]↦ (PureKObject.Pod updated_pure_pod) ∗
+        "Hown_child_keys" ∷ parent_key [[ γ_children ]]↦ owned_child_keys ∗
+        "Hown_grandchild_keys" ∷ key [[ γ_children ]]↦ owned_grandchild_keys
       ) ∨
-      "own_child_keys" ∷ parent_key [[ γ_children ]]↦ (owned_child_keys ∖ {[key]}))
+      "Hown_child_keys" ∷ parent_key [[ γ_children ]]↦ (owned_child_keys ∖ {[key]}))
   }}}.
 Proof.
   wp_start as "H". iNamed "H".
-  wp_apply wp_with_defer.
-  iIntros (defer) "defer". simpl subst. wp_auto. iRename "key" into "key_ptr".
+  wp_apply wp_with_defer. iIntros (defer) "Hdefer". simpl subst. wp_auto.
   wp_apply wp_globals_get.
   wp_apply wp_Mutex__Lock; [done|].
-  iIntros "[own_Mutex H]". iNamed "H". wp_auto.
+  iIntros "[Hown_Mutex H]". iNamed "H". wp_auto.
   wp_apply wp_globals_get. wp_apply wp_globals_get.
-  iAssert (⌜ abs_state !! key = Some (PureKObject.Pod owned_pod) ⌝%I) with "[own_pod own_abs]" as "%key_in_abs".
-  { iDestruct (map_valid with "own_abs own_pod") as %Hlookup. iPureIntro; exact Hlookup. }
-  iAssert (⌜ children !! parent_key = Some owned_child_keys ⌝%I) with "[own_children own_child_keys]" as "%parent_key_in_children".
-  { iDestruct (map_valid with "own_children own_child_keys") as %Hlookup. iPureIntro; exact Hlookup. }
-  iAssert (⌜ children !! key = Some owned_grandchild_keys ⌝%I) with "[own_children own_grandchild_keys]" as "%key_in_children".
-  { iDestruct (map_valid with "own_children own_grandchild_keys") as %Hlookup. iPureIntro; exact Hlookup. }
-  iAssert (⌜ ∃ obj, phys_state !! key = Some obj ⌝%I) with "[phys_abs_rep]" as "%key_in_phys".
+  iAssert (⌜ abs_state !! key = Some (PureKObject.Pod pure_pod) ⌝%I) as "%Hkey_in_abs".
+  { iDestruct (map_valid with "Hown_abs Hown_pod") as %Hlookup. iPureIntro; done. }
+  iAssert (⌜ children !! parent_key = Some owned_child_keys ⌝%I) as "%Hparent_key_in_children".
+  { iDestruct (map_valid with "Hown_children Hown_child_keys") as %Hlookup. iPureIntro; done. }
+  iAssert (⌜ children !! key = Some owned_grandchild_keys ⌝%I) as "%Hkey_in_children".
+  { iDestruct (map_valid with "Hown_children Hown_grandchild_keys") as %Hlookup. iPureIntro; done. }
+  iAssert (⌜ ∃ obj, phys_state !! key = Some obj ⌝%I) as "%Hkey_in_phys".
   {
-    iDestruct (big_sepM2_lookup_r with "phys_abs_rep") as (obj key_in_phys) "_".
-    { exact key_in_abs. }
-    iPureIntro. exists obj. exact key_in_phys.
+    iDestruct (big_sepM2_lookup_r with "Hphys_abs_rep") as (obj Hkey_in_phys) "_"; [done|].
+    iPureIntro. exists obj. done.
   }
-  destruct key_in_phys as [obj key_in_phys].
-  iDestruct (big_sepM2_split_singleton _ key _ _ phys_state abs_state key_in_phys key_in_abs with "phys_abs_rep") as "[k_rep other_rep]".
-  destruct decide_kind_is_pod with (KKey.Kind' key) as [kind_is_pod kind_is_not_replicaset].
-  { done. }
-  iAssert (∃ (ptr: loc) (pod: v1.Pod.t), pod_rep key obj (PureKObject.Pod owned_pod) ptr pod)%I 
-  with "[k_rep]" as "(%ptr & %pod & pod_rep)".
+  destruct Hkey_in_phys as [obj Hkey_in_phys].
+  iDestruct (big_sepM2_split_singleton _ key _ _ phys_state abs_state Hkey_in_phys Hkey_in_abs
+    with "Hphys_abs_rep") as "[Hk_rep Hother_rep]".
+  destruct decide_kind_is_pod with (KKey.Kind' key) as [kind_is_pod kind_is_not_replicaset]; [done|].
+  iAssert (∃ ptr v1 v2, pod_rep key obj (PureKObject.Pod pure_pod) ptr v1 v2)%I
+  with "[Hk_rep]" as "(%ptr & %pod & Hpod_rep)".
   { unfold obj_rep. rewrite kind_is_pod. done. }
-  iNamed "pod_rep".
-  inversion abs_v_is_pod as [Heq]. symmetry in Heq. subst. clear abs_v_is_pod.
-  wp_apply (wp_map_get with "[$own_phys]"). iIntros "own_phys". wp_auto.
-  rewrite /is_Some key_in_phys. wp_auto.
-  wp_apply wp_Accessor.
-  { done. }
-  iIntros (ret err) "(-> & ->)". wp_auto.
+  iNamed "Hpod_rep".
+  injection Habs_v_is_pod as Heq. subst v2.
+  wp_apply (wp_map_get with "[$Hown_phys]"). iIntros "Hown_phys". wp_auto.
+  rewrite /is_Some Hkey_in_phys. wp_auto.
+  wp_apply wp_Accessor; [done|].
   assert ((bool_decide (interface.nil = interface.nil)) = true) as nil_is_nil.
   { rewrite bool_decide_true //. }
   rewrite nil_is_nil. wp_auto.
-  iDestruct (struct_fields_split with "pod_ptr") as "H". iNamed "H".
+  iDestruct (struct_fields_split with "Hpod_ptr") as "H". iNamed "H".
   wp_apply (wp_GetFinalizers with "[$HObjectMeta]").
   iIntros (finalizers) "(-> & HObjectMeta)". wp_auto.
   wp_if_destruct.
@@ -84,7 +78,7 @@ Proof.
     iIntros (deletion_timestamp) "(-> & HObjectMeta)". wp_auto.
     wp_if_destruct.
     + wp_apply v1.wp_Now.
-      iIntros (time) "_". wp_auto.
+      iIntros (time pure_time) "Hdeepown_time". wp_auto.
       wp_apply (wp_SetDeletionTimestamp with "[$HObjectMeta]").
       iIntros (meta') "(-> & HObjectMeta)". wp_auto. wp_bind.
       wp_apply wp_globals_get.
@@ -94,39 +88,48 @@ Proof.
       wp_apply (wp_SetResourceVersion with "[$HObjectMeta]").
       iIntros (meta') "(-> & HObjectMeta)". wp_auto.
       iDestruct (struct_fields_combine (v:=v1.Pod.mk _ _ _ _)
-        with "[$HTypeMeta $HObjectMeta $HSpec $HStatus]") as "pod_ptr". simpl.
-      iDestruct (rename_pod with "pod_ptr") as "(%updated_pod & pod_ptr & %updated_pod_eq)".
-      iMod (auth_map.map_update _ _ (PureKObject.Pod updated_pod) with "own_abs own_pod")
-        as "[own_abs own_pod]".
-      iAssert (state_rep phys_state (<[key:=PureKObject.Pod updated_pod]> abs_state) %I)
-      with "[pod_ptr other_rep]" as "phys_abs_rep".
+        with "[$HTypeMeta $HObjectMeta $HSpec $HStatus]") as "Hpod_ptr". simpl.
+      iDestruct (rename_pod with "Hpod_ptr") as "(%updated_pod & Hpod_ptr & %Hupdated_pod_eq)".
+      set updated_pure_meta := pure_pod.(PurePod.ObjectMeta')
+        <| PureObjectMeta.ResourceVersion' := rv_str |>
+        <| PureObjectMeta.DeletionTimestamp' := Some pure_time |>.
+      set updated_pure_pod := pure_pod <| PurePod.ObjectMeta' := updated_pure_meta |>.
+      iMod (auth_map.map_update _ _ (PureKObject.Pod updated_pure_pod) with "Hown_abs Hown_pod")
+        as "[Hown_abs Hown_pod]".
+      iAssert (state_rep phys_state (<[key:=PureKObject.Pod updated_pure_pod]> abs_state) %I)
+      with "[Hpod_ptr Hother_rep Hdeepown_pod Hdeepown_time now]" as "Hphys_abs_rep".
       {
-        assert (delete key abs_state = delete key (<[key:=PureKObject.Pod updated_pod]> abs_state)) as ->.
+        assert (delete key abs_state = delete key (<[key:=PureKObject.Pod updated_pure_pod]> abs_state)) as ->.
         { rewrite delete_insert_eq. reflexivity. }
-        iAssert (("%namespace_match" ∷ ⌜ updated_pod.(v1.Pod.ObjectMeta').(v1.ObjectMeta.Namespace') = (KKey.Namespace' key) ⌝ ∗
-                  "%name_match" ∷ ⌜ updated_pod.(v1.Pod.ObjectMeta').(v1.ObjectMeta.Name') = (KKey.Name' key) ⌝ ∗
-                  "#PurePod.well_formed" ∷ PurePod.well_formed updated_pod)%I)
-        as "(% & % & #PurePod.well_formed')".
+        iAssert ((⌜ updated_pure_pod.(PurePod.ObjectMeta').(PureObjectMeta.Namespace') = (KKey.Namespace' key) ⌝ ∗
+                  ⌜ updated_pure_pod.(PurePod.ObjectMeta').(PureObjectMeta.Name') = (KKey.Name' key) ⌝ ∗
+                  ⌜ PurePod.well_formed updated_pure_pod ⌝)%I)
+        as "(%Hnamespace_match' & %Hname_match' & %well_formed')".
         {
           unfold PurePod.well_formed. unfold PureObjectMeta.well_formed.
           subst updated_pod. simpl. iFrame "#". done.
         }
-        iAssert (obj_rep key (interface.mk (ptrT.id v1.Pod.id) (# ptr)) (PureKObject.Pod updated_pod)%I)
-        with "[pod_ptr]" as "k_rep".
-        { unfold obj_rep. rewrite kind_is_pod. iExists ptr, updated_pod. unfold pod_rep. iFrame. iFrame "#". done. }
-        assert ((<[key:=PureKObject.Pod updated_pod]> abs_state) !! key = Some (PureKObject.Pod updated_pod)) as key_in_new_abs.
+        iAssert (PurePod.own updated_pod updated_pure_pod%I) with "[Hdeepown_pod Hdeepown_time now]" as "Hdeepown_pod'".
+        { iNamed "Hdeepown_pod". iFrame. iSplitR; [iPureIntro; rewrite Hupdated_pod_eq //|].
+          iNamed "Hown_objectmeta". rewrite Hupdated_pod_eq //.
+          iAssert (⌜ now_ptr ≠ null ⌝%I) as "%now_ptr_not_null".
+          { by iDestruct (typed_pointsto_not_null with "now") as %?. }
+          iFrame. iPureIntro. done. }
+        iAssert (obj_rep key (interface.mk (ptrT.id v1.Pod.id) (# ptr)) (PureKObject.Pod updated_pure_pod)%I)
+        with "[Hpod_ptr Hdeepown_pod']" as "Hk_rep".
+        { unfold obj_rep. rewrite kind_is_pod. iExists ptr, updated_pod, updated_pure_pod. unfold pod_rep. iFrame. done. }
+        iApply (big_sepM2_split_singleton _ key _ (PureKObject.Pod updated_pure_pod) phys_state (<[key:=PureKObject.Pod updated_pure_pod]> abs_state)
+          Hkey_in_phys with "[Hk_rep Hother_rep]").
         { rewrite lookup_insert. destruct (decide (key = key)) as [|Hcontra]; [reflexivity | contradiction]. }
-        iApply (big_sepM2_split_singleton _ key _ (PureKObject.Pod updated_pod) phys_state (<[key:=PureKObject.Pod updated_pod]> abs_state)
-          key_in_phys key_in_new_abs with "[k_rep other_rep]").
         iFrame.
       }
-      iAssert (kubernetes_state_consistent (dom used_uid) (<[key:=PureKObject.Pod updated_pod]> abs_state) children fresh_keys %I)
-      as "consistent'".
+      assert (ghost_well_formed (dom used_uid) (<[key:=PureKObject.Pod updated_pure_pod]> abs_state) children fresh_keys)
+      as Hghost_well_formed'.
       {
-        iNamed "consistent".
+        destruct Hghost_well_formed.
         assert (parent_key ≠ key) as parent_neq_key.
-        { specialize (no_self_parenting parent_key owned_child_keys key parent_key_in_children pod_is_child). done. }
-        assert (dom (<[key:=PureKObject.Pod updated_pod]> abs_state) = dom abs_state) as abs_dom_simpl.
+        { specialize (Hno_self_parenting parent_key owned_child_keys key Hparent_key_in_children Hpod_is_child). done. }
+        assert (dom (<[key:=PureKObject.Pod updated_pure_pod]> abs_state) = dom abs_state) as abs_dom_simpl.
         {
           rewrite dom_insert_L.
           assert ({[key]} ∪ dom abs_state = dom abs_state) as union_eq.
@@ -134,286 +137,222 @@ Proof.
           rewrite union_eq.
           reflexivity.
         }
-        assert ((PureKObject.metadata (PureKObject.Pod updated_pod)).(v1.ObjectMeta.OwnerReferences') = (PureKObject.metadata (PureKObject.Pod owned_pod)).(v1.ObjectMeta.OwnerReferences'))
-        as updated_pod_owner_references_eq.
-        { simpl. subst updated_pod. simpl. reflexivity. }
-        assert ((PureKObject.metadata (PureKObject.Pod updated_pod)).(v1.ObjectMeta.UID') = (PureKObject.metadata (PureKObject.Pod owned_pod)).(v1.ObjectMeta.UID'))
-        as updated_pod_uid_eq.
-        { simpl. subst updated_pod. simpl. reflexivity. }
-        iSplitR; [|iSplitR; [|iSplitR; [|iSplitR; [|iSplitR; [|iSplitR; [|iSplitR; [|iSplitR; [|iSplitR; [|iSplitR; [|iSplitR ]]]]]]]]]].
-        { iPureIntro. set_solver. }
-        { iPureIntro. intros k s Hlookup. specialize (children_exist k s Hlookup). rewrite dom_insert_L. set_solver. }
-        { iPureIntro. apply parents_children_same_namespace. }
-        { iPureIntro. apply no_self_parenting. }
-        { iPureIntro. apply children_disjoint. }
-        { iPureIntro. rewrite dom_insert_L. set_solver. }
-        { iPureIntro. apply fresh_keys_reserved. }
-        {
-          iPureIntro.
-          intros k1 k2 obj1 obj2 Hlookup1 Hlookup2 Huid_eq.
+        assert ((PureKObject.metadata (PureKObject.Pod updated_pure_pod)).(PureObjectMeta.OwnerReferences') = (PureKObject.metadata (PureKObject.Pod pure_pod)).(PureObjectMeta.OwnerReferences'))
+        as updated_pure_pod_owner_references_eq.
+        { simpl. subst updated_pure_pod. simpl. reflexivity. }
+        assert ((PureKObject.metadata (PureKObject.Pod updated_pure_pod)).(PureObjectMeta.UID') = (PureKObject.metadata (PureKObject.Pod pure_pod)).(PureObjectMeta.UID'))
+        as updated_pure_pod_uid_eq.
+        { simpl. subst updated_pure_pod. simpl. reflexivity. }
+        apply mk.
+        - set_solver.
+        - intros k s Hlookup. specialize (Hchildren_exist k s Hlookup). rewrite dom_insert_L. set_solver.
+        - apply Hparents_children_same_namespace.
+        - apply Hno_self_parenting.
+        - apply Hchildren_disjoint.
+        - rewrite dom_insert_L. set_solver.
+        - apply Hfresh_keys_reserved.
+        - intros k1 k2 obj1 obj2 Hlookup1 Hlookup2 Huid_eq.
           rewrite lookup_insert_Some in Hlookup1.
           rewrite lookup_insert_Some in Hlookup2.
           destruct Hlookup1 as [(Hk1_eq & Hobj1_eq) | (Hk1_neq & Hlookup_obj1)];
           destruct Hlookup2 as [(Hk2_eq & Hobj2_eq) | (Hk2_neq & Hlookup_obj2)].
-          - subst k1 k2. done.
-          - subst k1. eapply no_duplicate_uid; [eauto|eauto|].
+          + subst k1 k2. done.
+          + subst k1. eapply Hno_duplicate_uid; [eauto|eauto|].
             rewrite -Huid_eq -Hobj1_eq. done.
-          - subst k2. eapply no_duplicate_uid; [eauto|eauto|].
+          + subst k2. eapply Hno_duplicate_uid; [eauto|eauto|].
             rewrite Huid_eq -Hobj2_eq. done.
-          - eapply no_duplicate_uid; [eauto|eauto|done].
-        }
-        {
-          iPureIntro.
-          intros k obj Hlookup.
+          + eapply Hno_duplicate_uid; [eauto|eauto|done].
+        - intros k obj Hlookup.
           rewrite lookup_insert_Some in Hlookup.
           destruct Hlookup as [(Hk_eq & Hobj_eq) | (Hk_neq & Hlookup_obj)].
-          - subst k obj. rewrite updated_pod_uid_eq. eapply existing_uid_is_used. done.
-          - eapply existing_uid_is_used. done.
-        }
-        {
-          iModIntro.
-          iIntros (k s parent child_key child) "(%Hlookup_children & %Hlookup_child & %Hlookup_parent & %Hchild_in_s)".
-          rewrite lookup_insert_Some in Hlookup_child.
-          rewrite lookup_insert_Some in Hlookup_parent.
-          destruct Hlookup_child as [(Heq_child & Hchild_eq) | (Hneq_child & Hlookup_child)];
-          destruct Hlookup_parent as [(Heq_parent & Hparent_eq) | (Hneq_parent & Hlookup_parent)].
-          - subst child_key k child parent.
-            exfalso. by apply (no_self_parenting key s key Hlookup_children Hchild_in_s).
-          - subst child_key child.
-            rewrite updated_pod_owner_references_eq. iApply "children_point_to_parent". done.
-          - subst k parent.
-            rewrite updated_pod_uid_eq. iApply "children_point_to_parent". done.
-          - iApply ("children_point_to_parent" $! k s parent child_key child). iPureIntro. done.
-        }
-        {
-          iModIntro.
-          iIntros (k s parent child_key child) "[(%Hlookup_children & %Hlookup_child & %Hlookup_parent) Hmeta]".
-          rewrite lookup_insert_Some in Hlookup_child.
-          rewrite lookup_insert_Some in Hlookup_parent.
-          destruct Hlookup_child as [(Heq_child & Hchild_eq) | (Hneq_child & Hlookup_child)];
-          destruct Hlookup_parent as [(Heq_parent & Hparent_eq) | (Hneq_parent & Hlookup_parent)].
-          - subst child_key k child parent.
-            rewrite updated_pod_owner_references_eq updated_pod_uid_eq.
-            iDestruct ("only_children_point_to_parent" $! key s (PureKObject.Pod owned_pod) key (PureKObject.Pod owned_pod)
-              with "[Hmeta]") as "%Hkey_in_s".
-            { iFrame "Hmeta". iPureIntro. split; [|split]; done. }
-            exfalso. by apply (no_self_parenting key s key Hlookup_children Hkey_in_s).
-          - subst child_key child.
-            rewrite updated_pod_owner_references_eq.
-            iApply ("only_children_point_to_parent" $! k s parent key (PureKObject.Pod owned_pod) with "[Hmeta]").
-            iFrame "Hmeta". iPureIntro. split; [|split]; done.
-          - subst k parent.
-            rewrite updated_pod_uid_eq.
-            iApply ("only_children_point_to_parent" $! key s (PureKObject.Pod owned_pod) child_key child with "[Hmeta]").
-            iFrame "Hmeta". iPureIntro. split; [|split]; done.
-          - iApply ("only_children_point_to_parent" $! k s parent child_key child with "[Hmeta]").
-            iFrame "Hmeta". iPureIntro. split; [|split]; done.
-        }
-        {
-          iModIntro.
-          iIntros (k obj uid) "%Hlookup".
+          + subst k obj. rewrite updated_pure_pod_uid_eq. eapply Hexisting_uid_is_used. done.
+          + eapply Hexisting_uid_is_used. done.
+        - intros key_p obj_p key_c obj_c s Hlookup_p Hlookup_c Hlookup_children.
+          rewrite lookup_insert_Some in Hlookup_p.
+          rewrite lookup_insert_Some in Hlookup_c.
+          split; [intros Hkey_in_s|intros Hobj_has_controller_parent_of];
+          destruct Hlookup_p as [(<- & <-) | (Hkey_p_neq & Hlookup_p)];
+          destruct Hlookup_c as [(<- & <-) | (Hkey_c_neq & Hlookup_c)].
+          + exfalso. by apply (Hno_self_parenting key s key Hlookup_children Hkey_in_s).
+          + rewrite updated_pure_pod_uid_eq. eapply Hchildren_point_to_parent; [done|done|done|done].
+          + unfold obj_has_controller_parent_of. rewrite updated_pure_pod_owner_references_eq.
+            eapply Hchildren_point_to_parent; [done|done|done|done].
+          + eapply Hchildren_point_to_parent; [done|done|done|done].
+          + rewrite updated_pure_pod_uid_eq in Hobj_has_controller_parent_of.
+            pose proof ((proj2 (Hchildren_point_to_parent _ _ _ _ _ Hkey_in_abs Hkey_in_abs Hlookup_children) Hobj_has_controller_parent_of)). done.
+          + rewrite updated_pure_pod_uid_eq in Hobj_has_controller_parent_of.
+            pose proof ((proj2 (Hchildren_point_to_parent _ _ _ _ _ Hkey_in_abs Hlookup_c Hlookup_children) Hobj_has_controller_parent_of)). done.
+          + unfold obj_has_controller_parent_of in Hobj_has_controller_parent_of.
+            rewrite updated_pure_pod_owner_references_eq in Hobj_has_controller_parent_of.
+            pose proof ((proj2 (Hchildren_point_to_parent _ _ _ _ _ Hlookup_p Hkey_in_abs Hlookup_children) Hobj_has_controller_parent_of)). done.
+          + pose proof ((proj2 (Hchildren_point_to_parent _ _ _ _ _ Hlookup_p Hlookup_c Hlookup_children) Hobj_has_controller_parent_of)). done.
+        - intros k obj kind name uid Hlookup Href.
           rewrite lookup_insert_Some in Hlookup.
-          destruct Hlookup as [(Hk_eq & Hobj_eq) | (Hk_neq & Hlookup_obj)].
-          - subst k obj. rewrite updated_pod_owner_references_eq.
-            iApply "parent_uid_is_used". done.
-          - iApply ("parent_uid_is_used" $! k obj uid). done.
-        }
+          destruct Hlookup as [(<- & <-) | (Hkey_neq & Hlookup)].
+          + unfold obj_has_controller_parent_of in Href.
+            rewrite updated_pure_pod_owner_references_eq in Href.
+            eapply Hparent_uid_is_used; [done|done].
+          + eapply Hparent_uid_is_used; [done|done].
       }
       wp_apply (wp_Mutex__Unlock _ (is_kubernetes_state_inner γ_state γ_children γ_fresh_keys)
-      with "[$own_Mutex state_m_addr state_used_uid_addr state_rvc_addr own_phys own_used_uid own_abs phys_abs_rep own_children own_fresh_keys]").
-      { iFrame. iFrame "#". }
-      iApply "HΦ". iFrame. iSplitR; [done|]. iLeft. iFrame.
-      iAssert (⌜ now_ptr ≠ null ⌝%I) with "[now]" as "%now_ptr_not_null".
-      { by iDestruct (typed_pointsto_not_null with "now") as %?. }
-      iPureIntro. subst updated_pod. done.
-    + iDestruct (struct_fields_combine (V:=v1.Pod.t) with "[$HTypeMeta $HObjectMeta $HSpec $HStatus]") as "pod_ptr".
-      iAssert (state_rep phys_state abs_state %I) with "[pod_ptr other_rep]" as "phys_abs_rep".
+      with "[$Hown_Mutex Hstate_m_addr Hstate_used_uid_addr Hstate_rvc_addr Hown_phys Hown_used_uid Hown_abs Hphys_abs_rep Hown_children Hown_fresh_keys]").
+      { iFrame. iFrame "#". done. }
+      iApply "HΦ". iLeft. iFrame. done.
+    + iDestruct (struct_fields_combine (V:=v1.Pod.t) with "[$HTypeMeta $HObjectMeta $HSpec $HStatus]") as "Hpod_ptr".
+      iAssert (⌜ pure_pod.(PurePod.ObjectMeta').(PureObjectMeta.DeletionTimestamp') ≠ None ⌝%I) as "%Hdeletiontimestamp_not_none".
+      {
+        iNamed "Hdeepown_pod". iNamed "Hown_objectmeta". iPureIntro. intros H. apply Hown_deletiontimestamp_none in H. done.
+      }
+      iAssert (state_rep phys_state abs_state %I) with "[Hpod_ptr Hother_rep Hdeepown_pod]" as "Hphys_abs_rep".
       {
         iApply big_sepM2_split_singleton; [done | done|]. iFrame. unfold obj_rep. rewrite kind_is_pod.
-        iExists ptr, owned_pod. iFrame. iFrame "#". done.
+        iExists ptr, pod, pure_pod. iFrame. iFrame "#". done.
       }
       wp_apply (wp_Mutex__Unlock _ (is_kubernetes_state_inner γ_state γ_children γ_fresh_keys)
-        with "[$own_Mutex state_m_addr state_used_uid_addr state_rvc_addr own_phys own_used_uid own_abs phys_abs_rep own_children own_fresh_keys]").
-      { iFrame. iFrame "#". }
-      iApply "HΦ". iSplitR; [done|]. iLeft. iFrame. done.
+        with "[$Hown_Mutex Hstate_m_addr Hstate_used_uid_addr Hstate_rvc_addr Hown_phys Hown_used_uid Hown_abs Hphys_abs_rep Hown_children Hown_fresh_keys]").
+      { iFrame. iFrame "#". done. }
+      iApply "HΦ". iLeft. iFrame. done.
   - wp_apply wp_globals_get.
-    wp_apply (wp_map_delete with "[$own_phys]").
-    iIntros "own_phys". wp_auto.
+    wp_apply (wp_map_delete with "[$Hown_phys]").
+    iIntros "Hown_phys". wp_auto.
     iDestruct (struct_fields_combine (V:=v1.Pod.t)
-      with "[$HTypeMeta $HObjectMeta $HSpec $HStatus]") as "pod_ptr".
-    iMod (auth_map.map_delete with "own_pod own_abs") as "own_abs".
-    iMod (auth_map.map_update _ _ (owned_child_keys ∖ {[key]}) with "own_children own_child_keys")
-      as "[own_children own_child_keys]".
-    iMod (auth_map.map_delete with "own_grandchild_keys own_children") as "own_children".
-    iAssert (state_rep (delete key phys_state) (delete key abs_state) %I) with "[other_rep]" as "phys_abs_rep".
+      with "[$HTypeMeta $HObjectMeta $HSpec $HStatus]") as "Hpod_ptr".
+    iMod (auth_map.map_delete with "Hown_pod Hown_abs") as "Hown_abs".
+    iMod (auth_map.map_update _ _ (owned_child_keys ∖ {[key]}) with "Hown_children Hown_child_keys")
+      as "[Hown_children Hown_child_keys]".
+    iMod (auth_map.map_delete with "Hown_grandchild_keys Hown_children") as "Hown_children".
+    iAssert (state_rep (delete key phys_state) (delete key abs_state) %I) with "[Hother_rep]" as "Hphys_abs_rep".
     { done. }
-    iAssert (kubernetes_state_consistent (dom used_uid) (delete key abs_state) (delete key (<[parent_key:=owned_child_keys ∖ {[key]}]> children)) fresh_keys %I)
-    as "consistent'".
+    assert (ghost_well_formed (dom used_uid) (delete key abs_state) (delete key (<[parent_key:=owned_child_keys ∖ {[key]}]> children)) fresh_keys) as Hghost_well_formed'.
     {
-      iNamed "consistent".
+      destruct Hghost_well_formed.
       assert (parent_key ≠ key) as parent_neq_key.
-      { specialize (no_self_parenting parent_key owned_child_keys key parent_key_in_children pod_is_child). done. }
+      { specialize (Hno_self_parenting parent_key owned_child_keys key Hparent_key_in_children Hpod_is_child). done. }
       assert (dom (delete key (<[parent_key:=owned_child_keys ∖ {[key]}]> children)) = dom (delete key children) )
       as Hdom_children_eq.
       {
         assert (key ≠ parent_key) as key_neq_parent by (symmetry; exact parent_neq_key).
         rewrite !dom_delete_L dom_insert_L.
         assert (parent_key ∈ dom children) as parent_in_children_dom.
-        { apply elem_of_dom. exists owned_child_keys. exact parent_key_in_children. }
+        { apply elem_of_dom. exists owned_child_keys. exact Hparent_key_in_children. }
         assert ({[parent_key]} ∪ dom children = dom children) as union_eq.
         { set_solver. }
         rewrite union_eq.
         reflexivity.
       }
-      iSplitR; [|iSplitR; [|iSplitR; [|iSplitR; [|iSplitR; [|iSplitR; [|iSplitR; [|iSplitR; [|iSplitR; [|iSplitR; [|iSplitR ]]]]]]]]]].
-      { iPureIntro. set_solver. }
-      {
-        iPureIntro. intros k s Hlookup.
+      apply mk.
+      - set_solver.
+      - intros k s Hlookup.
         rewrite lookup_delete_Some lookup_insert_Some in Hlookup.
         destruct Hlookup as (Hk_neq_key & [(Hk_eq & Hs_eq) | (Hk_neq_parent & Hlookup)]).
-        - subst k s. rewrite dom_delete_L.
+        + subst k s. rewrite dom_delete_L.
           assert (owned_child_keys ⊆ dom abs_state) as owned_children_in_abs.
-          { apply children_exist with (k := parent_key). exact parent_key_in_children. }
+          { apply Hchildren_exist with (k := parent_key). exact Hparent_key_in_children. }
           set_solver.
-        - rewrite dom_delete_L.
-          assert (s ⊆ dom abs_state) as s_in_abs by (apply children_exist with (k := k); exact Hlookup).
+        + rewrite dom_delete_L.
+          assert (s ⊆ dom abs_state) as s_in_abs by (apply Hchildren_exist with (k := k); exact Hlookup).
           assert (s ## owned_child_keys) as s_disj_owned.
-          { destruct (decide (k = parent_key)); [congruence|]. eapply children_disjoint; done. }
+          { destruct (decide (k = parent_key)); [congruence|]. eapply Hchildren_disjoint; done. }
           assert (key ∉ s) as key_not_in_s.
-          { intros Hcontra. assert (key ∈ owned_child_keys) by exact pod_is_child. set_solver. }
+          { intros Hcontra. assert (key ∈ owned_child_keys) by exact Hpod_is_child. set_solver. }
           set_solver.
-      }
-      {
-        iPureIntro. intros k s child_key Hlookup Hchild_in_s.
+      - intros k s child_key Hlookup Hchild_in_s.
         rewrite lookup_delete_Some lookup_insert_Some in Hlookup.
         destruct Hlookup as (Hk_neq_key & [(Hk_eq & Hs_eq) | (Hk_neq_parent & Hlookup)]).
-        - subst k s. eapply parents_children_same_namespace; [exact parent_key_in_children | set_solver].
-        - eapply parents_children_same_namespace; done.
-      }
-      {
-        iPureIntro. intros k s child_key Hlookup Hchild_in_s.
+        + subst k s. eapply Hparents_children_same_namespace; [exact Hparent_key_in_children | set_solver].
+        + eapply Hparents_children_same_namespace; done.
+      -
+        intros k s child_key Hlookup Hchild_in_s.
         rewrite lookup_delete_Some lookup_insert_Some in Hlookup.
         destruct Hlookup as (Hk_neq_key & [(Hk_eq & Hs_eq) | (Hk_neq_parent & Hlookup)]).
-        - subst k s. eapply no_self_parenting; [exact parent_key_in_children | set_solver].
-        - eapply no_self_parenting; done.
-      }
-      {
-        iPureIntro. intros k1 s1 k2 s2 Hk1_neq_k2 Hlookup1 Hlookup2.
+        + subst k s. eapply Hno_self_parenting; [exact Hparent_key_in_children | set_solver].
+        + eapply Hno_self_parenting; done.
+      - intros k1 s1 k2 s2 Hk1_neq_k2 Hlookup1 Hlookup2.
         rewrite lookup_delete_Some lookup_insert_Some in Hlookup1.
         rewrite lookup_delete_Some lookup_insert_Some in Hlookup2.
         destruct Hlookup1 as (Hk1_neq_key & [(Hk1_eq & Hs1_eq) | (Hk1_neq_parent & Hlookup1)]);
         [destruct Hlookup2 as (Hk2_neq_key & [(Hk2_eq & Hs2_eq) | (Hk2_neq_parent & Hlookup2)]) |
          destruct Hlookup2 as (Hk2_neq_key & [(Hk2_eq & Hs2_eq) | (Hk2_neq_parent & Hlookup2)])].
-        - subst k1 k2. contradiction.
-        - subst k1 s1.
+        + subst k1 k2. contradiction.
+        + subst k1 s1.
           assert (owned_child_keys ## s2) as disj_orig.
-          { apply children_disjoint with (k1 := parent_key) (k2 := k2); [|assumption|assumption].
+          { apply Hchildren_disjoint with (k1 := parent_key) (k2 := k2); [|assumption|assumption].
             intros Heq. subst. contradiction. }
           set_solver.
-        - subst k2 s2.
+        + subst k2 s2.
           assert (s1 ## owned_child_keys) as disj_orig.
-          { apply children_disjoint with (k1 := k1) (k2 := parent_key); [|assumption|assumption].
+          { apply Hchildren_disjoint with (k1 := k1) (k2 := parent_key); [|assumption|assumption].
             intros Heq. subst. contradiction. }
           set_solver.
-        - apply children_disjoint with (k1 := k1) (k2 := k2); assumption.
-      }
-      { iPureIntro. rewrite dom_delete_L. set_solver. }
-      { iPureIntro. apply fresh_keys_reserved. }
-      {
-        iPureIntro.
-        intros k1 k2 obj1 obj2 Hlookup1 Hlookup2 Huid_eq.
+        + apply Hchildren_disjoint with (k1 := k1) (k2 := k2); assumption.
+      - rewrite dom_delete_L. set_solver.
+      - apply Hfresh_keys_reserved.
+      - intros k1 k2 obj1 obj2 Hlookup1 Hlookup2 Huid_eq.
         rewrite lookup_delete_Some in Hlookup1.
         rewrite lookup_delete_Some in Hlookup2.
         destruct Hlookup1 as (Hk1_neq_key & Hlookup_obj1).
         destruct Hlookup2 as (Hk2_neq_key & Hlookup_obj2).
-        eapply no_duplicate_uid; [eauto|eauto|done].
-      }
-      {
-        iPureIntro.
-        intros k obj Hlookup.
+        eapply Hno_duplicate_uid; [eauto|eauto|done].
+      - intros k obj Hlookup.
         rewrite lookup_delete_Some in Hlookup.
         destruct Hlookup as (Hk_neq_key & Hlookup_obj).
-        eapply existing_uid_is_used. done.
-      }
-      {
-        iModIntro.
-        iIntros (k s parent child_key child) "(%Hchildren_lookup & %Hchild_lookup & %Hparent_lookup & %Hchild_in_s)".
-        rewrite lookup_delete_Some in Hchildren_lookup.
-        rewrite lookup_delete_Some in Hchild_lookup.
-        rewrite lookup_delete_Some in Hparent_lookup.
-        destruct Hchildren_lookup as (Hk_neq_key, Hchildren_lookup).
-        destruct Hchild_lookup as (Hchild_key_neq_key, Hchild_lookup).
-        destruct Hparent_lookup as (Hk_neq_key', Hparent_lookup).
-        rewrite lookup_insert_Some in Hchildren_lookup.
-        destruct Hchildren_lookup as [(Hk_eq, Hs_eq) | (Hk_neq_parent, Hchildren_lookup)].
-        - subst k s.
-          iApply ("children_point_to_parent" $! parent_key owned_child_keys parent child_key child).
-          iPureIntro. split; [|split; [|split]]; try done; set_solver.
-        - iApply ("children_point_to_parent" $! k s parent child_key child).
-          iPureIntro. split; [|split; [|split]]; done.
-      }
-      {
-        iModIntro.
-        iIntros (k s parent child_key child) "[(%Hchildren_lookup & %Hchild_lookup & %Hparent_lookup) Hmeta]".
-        rewrite lookup_delete_Some in Hchildren_lookup.
-        rewrite lookup_delete_Some in Hchild_lookup.
-        rewrite lookup_delete_Some in Hparent_lookup.
-        destruct Hchildren_lookup as (Hk_neq_key, Hchildren_lookup).
-        destruct Hchild_lookup as (Hchild_key_neq_key, Hchild_lookup).
-        destruct Hparent_lookup as (Hk_neq_key', Hparent_lookup).
-        rewrite lookup_insert_Some in Hchildren_lookup.
-        destruct Hchildren_lookup as [(Hk_eq, Hs_eq) | (Hk_neq_parent, Hchildren_lookup)].
-        - subst k s.
-          iDestruct ("only_children_point_to_parent" $! parent_key owned_child_keys parent child_key child
-            with "[Hmeta]") as "%Hchild_in_owned".
-          { iFrame "Hmeta". iPureIntro. split; [|split]; done. }
-          iPureIntro. set_solver.
-        - iDestruct ("only_children_point_to_parent" $! k s parent child_key child
-            with "[Hmeta]") as "%Hchild_in_s".
-          { iFrame "Hmeta". iPureIntro. split; [|split]; done. }
-          iPureIntro. exact Hchild_in_s.
-      }
-      {
-        iModIntro.
-        iIntros (k obj uid) "%Hlookup".
+        eapply Hexisting_uid_is_used. done.
+      - intros key_p obj_p key_c obj_c s Hlookup_p Hlookup_c Hlookup_children.
+        rewrite lookup_delete_Some in Hlookup_children.
+        rewrite lookup_delete_Some in Hlookup_p.
+        rewrite lookup_delete_Some in Hlookup_c.
+        split;
+        destruct Hlookup_children as [Hkey_p_neq Hlookup_children];
+        destruct Hlookup_p as [Hkey_p_neq' Hlookup_p];
+        destruct Hlookup_c as [Hkey_c_neq Hlookup_c];
+        rewrite lookup_insert_Some in Hlookup_children;
+        destruct Hlookup_children as [(<- & <-) | (Hkey_p_neq'', Hlookup_children)].
+        + intros Hkey_c_in_s.
+          eapply Hchildren_point_to_parent; [done|done|done|set_solver].
+        + intros Hkey_c_in_s.
+          eapply Hchildren_point_to_parent; [done|done|done|done].
+        + intros Hobj_has_controller_parent_of.
+          pose proof ((proj2 (Hchildren_point_to_parent _ _ _ _ _ Hlookup_p Hlookup_c Hparent_key_in_children) Hobj_has_controller_parent_of)).
+          set_solver.
+        + intros Hobj_has_controller_parent_of.
+          pose proof ((proj2 (Hchildren_point_to_parent _ _ _ _ _ Hlookup_p Hlookup_c Hlookup_children) Hobj_has_controller_parent_of)). done.
+      - intros k obj kind name uid Hlookup.
         rewrite lookup_delete_Some in Hlookup.
         destruct Hlookup as (Hk_neq_key & Hlookup_obj).
-        iApply ("parent_uid_is_used" $! k obj uid). done.
-      }
+        eapply Hparent_uid_is_used. done.
     }
     wp_apply (wp_Mutex__Unlock _ (is_kubernetes_state_inner γ_state γ_children γ_fresh_keys)
-      with "[$own_Mutex state_m_addr state_used_uid_addr state_rvc_addr own_phys own_used_uid own_abs phys_abs_rep own_children own_fresh_keys]").
-    { iFrame. iFrame "#". }
-    iApply "HΦ". iFrame. done.
+      with "[$Hown_Mutex Hstate_m_addr Hstate_used_uid_addr Hstate_rvc_addr Hown_phys Hown_used_uid Hown_abs Hphys_abs_rep Hown_children Hown_fresh_keys]").
+    { iFrame. iFrame "#". done. }
+    iApply "HΦ". iFrame.
     Unshelve.
     done.
 Qed.
 
 Lemma wp_PodDelete_ptsto_mut namespace name
-  γ_state γ_children γ_fresh_keys owned_pod parent_key owned_child_keys owned_grandchild_keys:
+  γ_state γ_children γ_fresh_keys pure_pod parent_key owned_child_keys owned_grandchild_keys:
   {{{ is_pkg_init apimodel ∗
       "#inv" ∷ is_kubernetes_state γ_state γ_children γ_fresh_keys ∗
-      "own_pod" ∷ (mk_pod_key namespace name) [[ γ_state ]]↦ (PureKObject.Pod owned_pod) ∗
-      "own_child_keys" ∷ parent_key [[ γ_children ]]↦ owned_child_keys ∗
-      "own_grandchild_keys" ∷ (mk_pod_key namespace name) [[ γ_children ]]↦ owned_grandchild_keys ∗
-      "%pod_is_child" ∷ ⌜ (mk_pod_key namespace name) ∈ owned_child_keys ⌝
+      "Hown_pod" ∷ (mk_pod_key namespace name) [[ γ_state ]]↦ (PureKObject.Pod pure_pod) ∗
+      "Hown_child_keys" ∷ parent_key [[ γ_children ]]↦ owned_child_keys ∗
+      "Hown_grandchild_keys" ∷ (mk_pod_key namespace name) [[ γ_children ]]↦ owned_grandchild_keys ∗
+      "%Hpod_is_child" ∷ ⌜ (mk_pod_key namespace name) ∈ owned_child_keys ⌝
   }}}
     @! apimodel.PodDelete #namespace #name
-  {{{ (err: error.t) pod, RET #err;
-      "err_is_nil" ∷ ⌜ err = interface.nil ⌝ ∗
+  {{{ updated_pure_pod, RET #interface.nil;
       "pod_updated_or_deleted" ∷ ("pod_updated" ∷ (
-        "own_pod" ∷ (mk_pod_key namespace name) [[ γ_state ]]↦ (PureKObject.Pod pod) ∗
-        "own_child_keys" ∷ parent_key [[ γ_children ]]↦ owned_child_keys ∗
-        "own_grandchild_keys" ∷ (mk_pod_key namespace name) [[ γ_children ]]↦ owned_grandchild_keys ∗
-        "%deletiontimestamp_notnull" ∷ ⌜ pod.(v1.Pod.ObjectMeta').(v1.ObjectMeta.DeletionTimestamp') ≠ null ⌝
+        "%deletiontimestamp_notnull" ∷ ⌜ updated_pure_pod.(PurePod.ObjectMeta').(PureObjectMeta.DeletionTimestamp') ≠ None ⌝ ∗
+        "Hown_pod" ∷ (mk_pod_key namespace name) [[ γ_state ]]↦ (PureKObject.Pod updated_pure_pod) ∗
+        "Hown_child_keys" ∷ parent_key [[ γ_children ]]↦ owned_child_keys ∗
+        "Hown_grandchild_keys" ∷ (mk_pod_key namespace name) [[ γ_children ]]↦ owned_grandchild_keys
       ) ∨
-      "own_child_keys" ∷ parent_key [[ γ_children ]]↦ (owned_child_keys ∖ {[mk_pod_key namespace name]}))
+      "Hown_child_keys" ∷ parent_key [[ γ_children ]]↦ (owned_child_keys ∖ {[mk_pod_key namespace name]}))
   }}}.
 Proof.
   wp_start as "H". iNamed "H". wp_auto.
-  wp_apply (wp_objDelete_pod_ptsto_mut with "[$own_pod $own_child_keys $own_grandchild_keys]").
+  wp_apply (wp_objDelete_pod_ptsto_mut with "[$Hown_pod $Hown_child_keys $Hown_grandchild_keys]").
   { iFrame "#". done. }
-  iIntros (err pod) "H". iNamed "H". wp_auto. iApply "HΦ". iFrame.
+  iIntros (updated_pure_pod) "H". iNamed "H". wp_auto. iApply "HΦ". iFrame.
 Qed.
 
 End proof.
